---
course:
  - Applied Information Security
---
## Quick recap
Sender computes a ciphertextÂ $(c1,c2)$Â for messageÂ $m$Â with ephemeral randomÂ $r$:
- $c_1 = g^r \bmod p$
- $c_2 = m \cdot PK^r$ where $PK = g^x$ is the recipients public key.

Decryption (by holder of private keyÂ $x$) does:
- $s = c_1^x = g^{rx} = PK^r \bmod p$
- $m = c_2 \cdot s^{-1} \bmod p$
### ğŸ”‘ Recall how ElGamal encryption works

When theÂ **sender**Â encrypts a messageÂ `m`:

1. They choose a randomÂ **one-time random key**Â `r`.
    - This is a one-time random number.
    - It changes every time a message is encrypted, even if the recipient and the plaintext are the same.
2. They compute:
    - $c_1 = g^r \bmod p$
    - $c_2 = m \cdot PK^r \bmod p$
3. They sendÂ `(c1, c2)`Â as the ciphertext.

### ğŸ§® What happens in decryption?

The recipient knows:

- TheirÂ **private key**Â `x`
- The ciphertextÂ `(c1, c2)`

They compute the **shared secret**:

$s = {c_1}^x \bmod p$

SubstituteÂ `c1 = g^r`:

$$ s = (g^r)^x \bmod p = g^{rx} \bmod p $$

But recall the sender also computedÂ `PK^r = (g^x)^r = g^{xr}`Â during encryption.

So both sides end up with theÂ **same shared secretÂ `s`**Â without ever revealingÂ `r`Â orÂ `x`.